[WIP] added skel_extend
This lemma allows the code skeleton for both components in a forward simulation
to be replaced by a larger skeleton simultaneously, which gives us more
flexibility of choosing the skeleton for a composed transition system.

compcertox/Composition.v
@@ -44,17 +44,16 @@ Notation cmodule := (list Clight_.program).
 Fixpoint semantics (cmod: cmodule) sk: semantics li_c li_c :=
   match cmod with
   | nil => id_semantics sk
-  | (p :: nil) => Clight_.semantics1 p
   | (p :: ps) =>
     let L b := match b with
-               | true =>  semantics ps sk
-               | false => Clight_.semantics1 p
+               | true  => Clight_.semantics1 p
+               | false => semantics ps sk
                end
     in SmallstepLinking_.semantics L sk
   end.
 
 Notation cmod_combine := app.
-Notation " M ⊕ N " := (cmod_combine M N) (left associativity, at level 50).
+Notation " M ++ N " := (cmod_combine M N).
 
 Definition layer_comp {K} (M: cmodule) (L: layer K) sk :=
   comp_semantics' (semantics M sk @ K) L sk.
@@ -90,15 +89,189 @@ Proof.
   eapply compose_forward_simulations; eauto.
 Qed.
 
+Definition skel_extend {liA liB} (L: Smallstep_.semantics liA liB) sk :=
+  {|
+    activate se := L se;
+    skel := sk;
+    footprint := footprint L;
+  |}.
+
+Section SKEL.
+  Context {liA1 liB1 liA2 liB2}
+          {cc1: callconv liA1 liA2}
+          {cc2: callconv liB1 liB2}
+          {L1: Smallstep_.semantics liA1 liB1}
+          {L2: Smallstep_.semantics liA2 liB2}
+          (HL: forward_simulation cc1 cc2 L1 L2).
+  Variable (sk: AST.program unit unit).
+  Hypothesis Hsk: linkorder (skel L1) sk.
+
+  Lemma skel_extend_fsim:
+    forward_simulation cc1 cc2 (skel_extend L1 sk) (skel_extend L2 sk).
+  Proof.
+    unfold skel_extend. destruct HL.
+    constructor. econstructor. reflexivity.
+    - intros; cbn. eapply fsim_footprint. apply X.
+    - intros. exploit (fsim_lts X); eauto. cbn in *.
+      eapply Genv.valid_for_linkorder; eauto.
+    - apply (fsim_order_wf X).
+  Qed.
+End SKEL.
+
+Section HCOMP_INIT_STATE.
+  Context {li} (L1 L2: Smallstep_.semantics li li).
+  Let L := fun i => match i with | true => L1 | false => L2 end.
+  Hypothesis H: forall i q s se, Smallstep_.initial_state (L i se) q s ->
+                            valid_query (L i) se q.
+
+  Lemma initial_state_valid_comp sk:
+    forall q s se,
+      Smallstep_.initial_state (SmallstepLinking_.semantics L sk se) q s ->
+      valid_query (SmallstepLinking_.semantics L sk) se q.
+  Proof.
+    intros q s se Hx. inv Hx. destruct i.
+    - exploit H; eauto. firstorder.
+    - exploit H; eauto. firstorder.
+  Qed.
+End HCOMP_INIT_STATE.
+
+Lemma cmodule_initial_state_valid sk M:
+  (List.length M >= 1)%nat ->
+  forall se s q, Smallstep_.initial_state (semantics M sk se) q s ->
+            valid_query (semantics M sk) se q.
+Proof.
+  set (P := fun M => forall se s q, Smallstep_.initial_state (semantics M sk se) q s -> valid_query (semantics M sk) se q).
+  apply (@list_ind1 _ P); subst P; cbn beta.
+  - intros. inv H. destruct H0 as (? & ? & ? & ?). destruct i.
+    + unfold valid_query. split; auto.
+      eexists; split; eauto. now left.
+    + inv H0.
+  - intros p ps IH se s q H.
+    cbn. eapply initial_state_valid_comp.
+    * intros. destruct i.
+      eapply initial_state_valid; eauto.
+      eapply IH; eauto.
+    * apply H.
+Qed.
+
+(* TODO: move this to lifting.v *)
+Lemma lifting_step_star {liA liB K} (L: Smallstep_.semantics liA liB) se qset s1 t s2 k:
+  Star (L se) qset s1 t s2 ->
+  Star(lifted_lts K (L se)) qset (s1, k) t (s2, k).
+Proof.
+  induction 1; [eapply star_refl | eapply star_step]; eauto.
+  constructor; auto.
+Qed.
+
+Lemma lifting_step_plus {liA liB K} (L: Smallstep_.semantics liA liB) se qset s1 t s2 k:
+  Plus (L se) qset s1 t s2 ->
+  Plus (lifted_lts K (L se)) qset (s1, k) t (s2, k).
+Proof.
+  destruct 1; econstructor; eauto using lifting_step_star.
+  split; eauto.
+Qed.
+
+Lemma lifting_simulation {K li1 li2} {L1 L2: Smallstep_.semantics li1 li2}:
+  L1 ≤ L2 -> L1 @ K ≤ L2 @ K.
+Proof.
+  intros [H]. constructor.
+  eapply Forward_simulation with
+      (fsim_order H)
+      (fun se1 se2 w i '(s1, k1) '(s2, k2) =>
+         fsim_match_states H se1 se2 w i s1 s2 /\ k1 = k2).
+  - apply (fsim_skel H).
+  - intros i. apply (fsim_footprint H).
+  - destruct H as [? ? ? ? ? Hf ?]. cbn. clear -Hf.
+    intros se1 se2 [ ] qset Hse Hse'.
+    specialize (Hf se1 se2 tt qset Hse Hse'). subst.
+    econstructor.
+    + intros [q kq] ? [s1 ks] [ ] Hi. inv Hi. cbn in *; subst.
+      exploit (fsim_match_initial_states Hf); eauto. econstructor.
+      intros (? & ? & ? & ?). eexists _, (_, _).
+      repeat apply conj; cbn; eauto.
+    + intros i [s1 ks1] [s2 ks2] [r kr] [Hs Hk] Hi.
+      inv Hi. cbn in *; subst.
+      exploit (fsim_match_final_states Hf); eauto.
+      intros (? & ? & ?). inv H1.
+      eexists (_, _). repeat apply conj; cbn; eauto.
+    + intros i [s1 ks1] [s2 ks2] [q1 kq1] [Hs Hk] Hi.
+      inv Hi. cbn in *; subst.
+      exploit (fsim_match_external Hf); eauto.
+      intros (? & ? & ? & Hq & ? & Hx). inv Hq.
+      eexists tt, (_, _). repeat apply conj; cbn; eauto.
+      intros [r kr] [? ?] [s1' Hs1'] <- Ha. inv Ha.
+      cbn in *; subst. exploit Hx; eauto.
+      intros (? & ? & ? & ?). eexists _, (_, _).
+      repeat apply conj; cbn; eauto.
+    + intros [s1 ks1] t [s1' ks1'] Hstep i [s2 ks2] [Hs Hk].
+      inv Hstep. exploit (fsim_simulation Hf); eauto.
+      intros (? & ? & Hx & ?). destruct Hx.
+      * eexists _, (_, _); repeat apply conj; eauto.
+        left. apply lifting_step_plus; auto.
+      * eexists _, (_, _); repeat apply conj; eauto.
+        right. destruct H1. split; eauto using lifting_step_star.
+  - apply fsim_order_wf.
+Qed.
+
+Section HCOMP_FSIM.
+
+  Context {li1 li2} (cc: callconv li1 li2)
+          (L1a L1b: Smallstep_.semantics li1 li1)
+          (L2a L2b: Smallstep_.semantics li2 li2).
+  Hypothesis (HL1: forward_simulation cc cc L1a L2a)
+             (HL2: forward_simulation cc cc L1b L2b).
+  Let L1 := fun b => match b with | true => L1a | false => L1b end.
+  Let L2 := fun b => match b with | true => L2a | false => L2b end.
+
+  Variable (sk: AST.program unit unit).
+  Hypothesis (Hsk1: linkorder (skel L1a) sk)
+             (Hsk2: linkorder (skel L1b) sk).
+
+  Lemma horizontal_compose_simulation':
+    forward_simulation cc cc (SmallstepLinking_.semantics L1 sk)
+                       (SmallstepLinking_.semantics L2 sk).
+  Proof.
+    destruct HL1 as [Ha]. destruct HL2 as [Hb].
+    assert (HL: forall i, fsim_components cc cc (L1 i) (L2 i)) by (intros [|]; auto).
+    constructor.
+    eapply Forward_simulation with
+        (SmallstepLinking_.order cc L1 L2 HL)
+        (SmallstepLinking_.match_states cc L1 L2 HL).
+    - reflexivity.
+    - intros i. cbn. destruct Ha, Hb.
+      rewrite fsim_footprint, fsim_footprint0. reflexivity.
+    - intros se1 se2 w qset Hse Hse1.
+      eapply SmallstepLinking_.semantics_simulation; eauto.
+      intros [|]; cbn; eapply Genv.valid_for_linkorder; eauto.
+    - clear - HL. intros [i x].
+      induction (fsim_order_wf (HL i) x) as [x Hx IHx].
+      constructor. intros z Hxz. inv Hxz; SmallstepLinking_.subst_dep. eauto.
+  Qed.
+End HCOMP_FSIM.
+
+Lemma singleton_app {A} x (xs: list A):
+  app (x :: nil) xs = x :: xs.
+Proof. firstorder. Qed.
+
 (* M has to be non-empty is due to the fact that we can't prove id ∘ L ≡ L *)
 Lemma cmodule_simulation {M N : cmodule} {sk1 sk2 sk: AST.program unit unit}:
-  (* (List.length M >= 1)%nat -> *)
-  comp_semantics' (semantics M sk1) (semantics N sk2) sk ≤ semantics (M ⊕ N) sk.
+  (List.length N >= 1)%nat -> (List.length M >= 1)%nat ->
+  comp_semantics' (semantics M sk1) (semantics N sk2) sk ≤ semantics (M ++ N) sk.
 Proof.
-  (* set (P := fun l => comp_semantics' (semantics l sk1) (semantics N sk2) sk ≤ semantics (l ⊕ N) sk). *)
-  (* apply (@list_ind1 _ P); subst P; cbn beta. *)
-  (* - intros p. etransitivity. *)
-  (*   apply categorical_compose_approximation. *)
+  intros HN.
+  set (P := fun l => comp_semantics' (semantics l sk1) (semantics N sk2) sk ≤ semantics (l ++ N) sk).
+  apply (@list_ind1 _ P); subst P; cbn beta.
+  - intros p. etransitivity.
+    apply categorical_compose_approximation.
+    {
+      intros [|] se q s H.
+      - eapply cmodule_initial_state_valid; eauto.
+      - eapply cmodule_initial_state_valid; eauto.
+    }
+    rewrite singleton_app. cbn.
+    apply horizontal_compose_simulation'.
+    +
+
 Admitted.
 
 (* A special case of categorical_compose_simulation *)
@@ -117,18 +290,18 @@ Admitted.
 Lemma clight_krel {K1 K2} (R: rel_adt K1 K2) p:
   forward_simulation R R (Clight_.semantics1 p @ K1) (Clight_.semantics1 p @ K2).
 Proof.
-Admitted.
+  induction R; simpl.
+  - apply lifting_simulation.
+    apply identity_forward_simulation.
+  - apply clight_sim.
+  - eapply compose_forward_simulations; eauto.
+Qed.
 
 Lemma cmodule_krel {K1 K2} (R: rel_adt K1 K2) M sk:
   forward_simulation R R (semantics M sk @ K1) (semantics M sk @ K2).
 Proof.
 Admitted.
 
-Lemma lifting_simulation {K li1 li2}
-      {L1 L2: Smallstep_.semantics li1 li2}:
-  L1 ≤ L2 -> L1 @ K ≤ L2 @ K.
-Proof.
-Admitted.
 
 Section VCOMP.
 
@@ -136,7 +309,7 @@ Section VCOMP.
           {R: rel_adt K1 K2} {S: rel_adt K2 K3}
           (HL1: ksim L1 L2 M R) (HL2: ksim L2 L3 N S).
 
-  Theorem layer_vcomp: ksim L1 L3 (M ⊕ N) (R ∘ S).
+  Theorem layer_vcomp: ksim L1 L3 (M ++ N) (R ∘ S).
   Proof.
     unfold ksim in *.
     pose proof (cmodule_krel S M (skel L1)) as Hsim1.
